General clean-up.

PersistentArrays.v
@@ -29,7 +29,7 @@ Hint Unfold upd.
 
 (* 
    pa_model states that, given a pointer "p", we either have: 
-   1. p points to an array "Arr", with elements given by (Z -> Z)
+   1. p points to an array "Arr", with elements given by (N -> N)
    2. p points to different "Diff", which is a change of another valid array,
       in one position only, updating the other array in that position (using upd)
 *)
@@ -109,7 +109,8 @@ Proof.
   intros m p i v p' f f' pr1 pr2 pr3; subst; eapply pa_model_diff; eauto.
 Qed.
 
-(* Main separation lemma *)
+(* Separation lemma: allocating a new pointer on the heap has no
+   effect on existing PAs. *)
 Lemma pa_model_sep' :
   forall s t f v t',
     find s t' = None -> 
@@ -134,7 +135,8 @@ Inductive PAData : option data -> Prop :=
 
 Hint Constructors PAData.
 
-(* Main separation lemma *)
+(* Separation lemma: a pointer that does not point to a structure
+   of a PA, can be safely updated without affecting existing PAs  *)
 Lemma pa_model_sep_padata :
   forall s t f v t',
     ~ (PAData (find s t')) ->
@@ -162,7 +164,7 @@ Proof. intros; apply pa_model_sep'; auto. Qed.
 Lemma find_eqdec : forall {A} s p, sumbool (find s p = None) (exists (c : A), find s p = Some c).
 Proof. intros; destruct (find s p); eauto. Qed.
 
-Lemma pa_model_copy :
+Lemma pa_model_copy_fresh :
   forall s p f, pa_model s p f -> forall v, find s p = Some v -> 
            forall t, (forall (p' : M.key) (x : data), find s p' = Some x -> p' <> t) ->
                 pa_model (update s t v) t f.
@@ -179,7 +181,7 @@ Proof.
 Qed.
 
 Hint Resolve pa_model_fun pa_model_diff_2 pa_model_sep'
-             pa_model_sep_padata pa_model_copy.
+             pa_model_sep_padata pa_model_copy_fresh.
   
 (** set refinement **)
 
@@ -191,7 +193,7 @@ Proof.
   destruct vInPtr as [ f | j vInJ t' | ].
   - NEW (Arr (upd f i v)) res.
     WRITE ptr (Diff i (f i) res).
-    RETURN res; inversion X; subst; rewrite H in e1; inversion e1; eauto 6.
+    RETURN res; inversion X; subst; context_simpl; eauto 6.
   - unfold newRef.
     NEW (Diff i v ptr) res.
     RETURN res. 
@@ -200,7 +202,7 @@ Proof.
     destruct (find_eqdec pre res); auto; destruct e; exfalso; eapply n; eauto.
     apply pa_model_sep'; auto.
     destruct (find_eqdec pre res); auto; destruct e; exfalso; eapply n; eauto.
-  - RETURN ptr; auto; inversion X; subst; rewrite H in e; inversion e.
+  - RETURN ptr; inversion X; subst; context_simpl.
 Qed.
 
 (*** GET ***)
@@ -290,10 +292,8 @@ Lemma dist_fun : forall s ptr l1, dist s ptr l1 -> forall l2, dist s ptr l2 -> l
 Proof.
   intros s ptr l1 H.
   induction H; intros.
-  - inversion X; subst; auto.
-    rewrite e in H; inversion H.
-  - inversion X; subst; rewrite e in H0; inversion H0; subst.
-    apply f_equal; auto.
+  - inversion X; context_simpl; auto.
+  - inversion X; context_simpl; apply f_equal; auto.
 Qed.
 
 Lemma dist_InT : forall s ptr l, dist s ptr l -> InT ptr l.
@@ -317,7 +317,9 @@ Qed.
 Lemma pa_model_dist : forall s ptr f, pa_model s ptr f -> { l : list Ptr & dist s ptr l }.
 Proof. intros; induction X; eauto. destruct IHX; eauto. Qed.
 
-Lemma pa_model_sep_uglyT :
+(* Separation lemma: if a pointer does not belong to the a given PA,
+   then updating it should not affect that PA *)
+Lemma pa_model_sep :
   forall s f v ptr ptr' l,
     pa_model s ptr f ->
     dist s ptr l ->
@@ -326,11 +328,9 @@ Lemma pa_model_sep_uglyT :
 Proof.
   intros s f v ptr ptr' l HPA Hdist. generalize dependent ptr'. generalize dependent v. generalize dependent l.
   induction HPA; intros.
-  - apply pa_model_array.
-    rewrite findNUpdate; auto.
+  - apply pa_model_array; rewrite findNUpdate; auto.
     unfold not; intros; subst.
-    apply dist_InT in Hdist.
-    contradiction.
+    apply dist_InT in Hdist; contradiction.
   - apply pa_model_diff with (p' := p').
     rewrite findNUpdate; auto.
     unfold not; intros; subst.
@@ -339,7 +339,9 @@ Proof.
     eapply IHHPA with (l := l0); auto.
 Qed.
 
-Lemma pa_model_sep_ugly2T :
+(* Separation lemma: if a pointer does not belong to the a given PA,
+   then updating it to that PA should make it a PA as well *)
+Lemma pa_model_sep_copy :
   forall s f v ptr ptr' l,
     pa_model s ptr f ->
     dist s ptr l ->
@@ -350,21 +352,16 @@ Proof.
   intros s f v ptr ptr' l HPA Hdist HFind. generalize dependent ptr'. generalize dependent v. generalize dependent l.
   induction HPA; intros.
   - apply pa_model_array; rewrite e in H; now rewrite findUpdate.
-  - rewrite e in H.
-    apply pa_model_diff with (p' := p'). 
+  - rewrite e in H; apply pa_model_diff with (p' := p'). 
     rewrite findUpdate; auto.
     assert (Ha : pa_model s p' f) by assumption.
     apply pa_model_dist in HPA.
     destruct HPA.
-    eapply pa_model_sep_uglyT. auto.
-    apply d.
+    eapply pa_model_sep; eauto.
     assert (Ha1 : l = p :: x).
     inversion Hdist; subst; rewrite e in H0; inversion H0; subst.
-    apply f_equal.
-    eapply dist_fun; eauto.
-    subst.
-    unfold not; intros; apply HFind.
-    auto.
+    apply f_equal; eapply dist_fun; eauto.
+    subst; intros; auto.
 Qed.
 
 Lemma dist_wf : forall s p1 l, dist s p1 l -> forall p2, p1 <> p2 -> InT p2 l ->
@@ -416,7 +413,8 @@ Proof.
     eapply Nat.nlt_succ_diag_l; apply l0.
 Qed.
 
-(* Main separation lemma. *)
+(* When a pointer that points to (Diff i v t'), can be updated to whatever t'
+   points to *)
 Lemma pa_model_desc : forall s p1 f i v, pa_model s p1 (upd f i v) ->
                                     forall p2 v', pa_model s p2 f ->
                                              find s p1 = Some (Diff i v p2) ->
@@ -427,7 +425,7 @@ Proof.
   assert (Ha : pa_model s p2 f) by assumption.
   apply pa_model_dist in HP2.
   destruct HP2.
-  eapply pa_model_sep_ugly2T; eauto.
+  eapply pa_model_sep_copy; eauto.
 
   assert (Ha1 : pa_model s p1 (upd f i v)) by assumption.
   apply pa_model_dist in HP1.
@@ -463,7 +461,7 @@ Proof.
     apply e.
 Qed.
 
-Hint Resolve dist_sepT pa_model_dist pa_model_sep_uglyT pa_model_sep_ugly2T.
+Hint Resolve dist_sepT pa_model_dist pa_model_sep pa_model_sep_copy.
 Hint Resolve pa_model_desc pa_dist_sep_padata.
 
 Lemma dist_InT_find : forall ptr1 s l, dist s ptr1 l -> forall ptr2, InT ptr2 l ->
@@ -488,8 +486,6 @@ Proof.
 Qed.
 
 Hint Resolve dist_InT_find dist_InT_find_padata.
-
-(***** Latest changes ******)
 
 (* Given the root pointer "ptr" and an auxiliary traversal pointer "t",
   "t" points to a persistent array (modelled by some f) such that:
@@ -544,11 +540,11 @@ Proof.
   inversion X0; subst; eauto.
   NEW vInPtr t.
   NEW (ResultGet None) done.
-  unfold Inv; apply whileSpec.
+  WHILE (Inv ptr t done i) (fun s : S data => negb (data_get_eqb_some (find s done))); unfold Inv.
   - refine_simpl.
     exists s1.
     repeat split; auto.
-    * apply pa_model_sep'; eauto. auto.
+    * apply pa_model_sep'; eauto.
       destruct (find_eqdec (update s0 t vInPtr) done); eauto;
       destruct e; exfalso; eapply n; eauto.
     * assert (Ha1 : pa_model (update s0 t vInPtr) ptr s1).
@@ -564,21 +560,17 @@ Proof.
       destruct X0.
       exists x; split. 
       repeat apply dist_sepT; auto.
-      + intros.
-        assert (Ha2 : { v : data & find s0 t = Some v }) by eauto.
+      + intros; assert (Ha2 : { v : data & find s0 t = Some v }) by eauto.
         destruct Ha2 as [v HFind]; apply n0 in HFind; now apply HFind. 
-      + intros.
-        assert (Ha2 : { v : data & find s0 done = Some v }) by eauto.
+      + intros; assert (Ha2 : { v : data & find s0 done = Some v }) by eauto.
         destruct Ha2 as [v HFind].
         rewrite <- findNUpdate with (p' := t) (v := vInPtr) in HFind. 
         apply n in HFind; now apply HFind.
         unfold not; intros; subst.
         apply n0 in HFind; now apply HFind.
-      + intros.
-        assert (Ha2 : { v : data & find s0 t = Some v }) by eauto.
+      + intros; assert (Ha2 : { v : data & find s0 t = Some v }) by eauto.
         destruct Ha2 as [v HFind]; apply n0 in HFind; now apply HFind. 
-  - unfold Inv.
-    READ t vInT.
+  - READ t vInT.
     inversion p; eauto.
     destruct vInT.
     WRITE done (ResultGet (Some (n i))).
@@ -590,10 +582,8 @@ Proof.
     * exists s2; split; auto.
     * rewrite findUpdate; left; repeat apply f_equal.
       inversion p; rewrite e0 in H; inversion H; now subst.
-    * destruct (Nat.eq_dec i n).
-      + subst.
-        rewrite PeanoNat.Nat.eqb_refl.
-        WRITE done (ResultGet (Some n0)).
+    * ITE (i =? n).
+      + WRITE done (ResultGet (Some n0)).
         destruct s3; eauto.
         RETURN tt.
         eexists; split; eauto. 
@@ -602,10 +592,9 @@ Proof.
         now destruct (p1 _ X).
         eauto.
         rewrite findUpdate; left; repeat apply f_equal.
-        inversion p0; rewrite e0 in H; inversion H; subst.
-        unfold upd; now rewrite <- beq_nat_refl.
-      + apply Nat.eqb_neq in n1; rewrite n1.
-        READ p vInT'.
+        inversion p0; rewrite e0 in H; inversion H; subst. 
+        unfold upd; now rewrite <- Heqb.
+      + READ p vInT'.
         inversion p0; subst; rewrite e in H; inversion H; subst.
         inversion X; subst; eauto.
         WRITE t vInT'.
@@ -613,13 +602,13 @@ Proof.
         inversion p0; subst; rewrite e1 in H; inversion H; subst; clear H.
         exists f0.
         repeat split. eauto 2.
-        eapply pa_model_sep_uglyT; eauto 2; now destruct (p1 _ X0).
-        destruct (p1 _ X0); rewrite <- e; unfold upd; now rewrite n1. 
+        eapply pa_model_sep; eauto 2; now destruct (p1 _ X0).
+        destruct (p1 _ X0); rewrite <- e; unfold upd; now rewrite <- Heqb. 
         exists s2.
         split; auto; apply dist_sepT; auto.
-        destruct s3.
+        destruct s3. 
         left; rewrite findNUpdate; eauto 1.
-        rewrite e; repeat apply f_equal; unfold upd; now rewrite n1.
+        rewrite e; repeat apply f_equal; unfold upd; now rewrite <- Heqb.
         unfold not; intros; subst; rewrite e1 in e; inversion e.
         right; rewrite findNUpdate; eauto 1; unfold not; intros; subst;
         rewrite e1 in e; inversion e.
@@ -811,295 +800,6 @@ Inductive WhileL' (I : Type) (O : I -> Type) (a : Type) : Type :=
 
 (** STOP HERE **)
 
-(*
-Parameter N : nat.
 
-Inductive repr (f : nat -> nat) : nat -> nat -> Prop :=
-  | repr_zero : forall i, f i = i -> repr f i i
-  | repr_succ : forall i j r, f i = j -> 0 <= j < N -> ~ j = i -> repr f j r ->
-                         repr f i r.
-
-Definition reprf (f : nat -> nat) :=
-  (forall i, 0 <= i < N -> 0 <= f i < N) /\
-  (forall i, 0 <= i < N -> exists j, repr f i j).
-*)
-
-
-
-
-(* Attempt following Chargueraud's paper *)
-
-Definition Rank := nat.
-
-(* We know that Ptr will point to Content 
-   TODO maybe find a better translation for polymorphic references "ref a"? *)
-Definition Elem := Ptr.
-
-Inductive Content : Type :=
-  | Root : Rank -> Content
-  | Link : Elem -> Content.
-
-(** Make **)
-
-Definition make : unit -> WhileL Elem :=
-  fun => New 0 (fun ptr => Return ptr).
-
-Definition makeSpec : WhileL Elem.
-  refine (Spec _).
-  refine (Predicate (fun s => True) _).
-  intros s H t s'.
-  refine ({p : Ptr | find s' p = Some (dyn Rank 0)}).
-Defined.
-
-Lemma makeResult : makeSpec ⊑ make tt.
-Proof.
-  NEW 0 p.
-  apply returnStep.
-  unfold_refinements; refine_simpl; exists p; auto.
-Qed.
-
-(** Find/Link **)
-
-(* TODO the following 2 definitions should be used temporarly *)
-Definition addr_eqb (x : Addr.addr) (y : Addr.addr) :=
-  match x, y with
-    | Addr.MkAddr v1, Addr.MkAddr v2 => Nat.eqb v1 v2
-  end.
-
-Definition eqb_addr_spec : forall x y, reflect (x = y) (addr_eqb x y).
-  intros x y; destruct x; destruct y; simpl; apply iff_reflect; split; intros;
-  [ inversion H; now apply PeanoNat.Nat.eqb_eq
-  | apply f_equal; now apply PeanoNat.Nat.eqb_eq ].
-Defined.
-
-Definition linkByRank (x : Elem) (y : Elem) (rx : Rank) (ry : Rank) :
-  WhileL Elem :=
-  match Nat.compare rx ry with
-    | Lt => Write x (Link y) (Return y)
-    | Gt => Write y (Link x) (Return x)
-    | Eq => Write y (Link x) (Write y (Root (Nat.succ rx)) (Return x))
-  end.
-
-Definition link (x : Elem) (y : Elem) : WhileL Elem :=
-  if addr_eqb x y
-  then Return x
-  else let readPtrs k :=
-           Read x (fun xVal => Read y (fun yVal => k xVal yVal)) in
-       let cont (vx vy : Content) :=
-           match vx, vy with
-             | Root rx, Root ry => linkByRank x y rx ry
-             | _, => Return x (* hopefully during the refinement process
-                                     we can show this case will never occur *)
-           end in
-       readPtrs cont.
-
-(* I don't like this spec, it's too similar to the code *)
-Definition linkSpec (x : Elem) (y : Elem) : WhileL Elem.
-  refine (Spec _).
-  refine (Predicate (fun s => prod ({r : Rank | find s x =
-                                                  Some (dyn Content (Root r))})
-                                     ({r : Rank | find s y =
-                                                  Some (dyn Content (Root r))}))
-                    _).
-  intros s [[rx HxFind] [ry HyFind]] t s'.
-  destruct (eqb_addr_spec x y).
-  apply (t = x).
-  destruct (Nat.compare rx ry).
-  apply (prod (find s' x = Some (dyn Content (Link y))) (t = y)).
-  apply (prod (find s' y = Some (dyn Content (Link x))) (t = x)).
-  apply (prod (find s' y = Some (dyn Content (Link x)))
-              (prod (find s' x = Some (dyn Content (Root (Nat.succ rx))))
-                    (t = y))).
-Defined.
-
-(* The following does not pass Coq's termination checker *)
-
-Fixpoint ufind (x : Elem) : WhileL Elem.
-(* The following does not pass Coq's termination checker
-refine (
-  Read Elem Content x
-       (fun v => match v with
-                  | Root => Return x
-                  | Link y => bind (ufind y)
-                                   (fun z => Write x (Link z) (Return z))
-                end)). *)
-Admitted.
-
-(* TODO This accounts for paths but not for updated references *)
-Inductive PathToRoot (s : heap) (el : Elem) : list Elem -> Type :=
-  | This : forall v, find s el = Some (dyn Content (Root v)) ->
-                PathToRoot s el (el :: nil)
-  | Path : forall p r l, find s p = Some (dyn Content (Link r)) ->
-                    PathToRoot s el l -> 
-                    PathToRoot s el (r :: l).
-
-Definition findSpec (x : Elem) : WhileL Elem.
-  refine (Spec _).
-  refine (Predicate (fun s => { v : Content | find s x = Some (dyn Content v)}) _).
-  intros s [v HFindX] t s'.
-  refine ({ l : list Elem & prod (PathToRoot s x l)
-                                 (head (rev l) = Some t) } ).
-Defined.
-
-(** Union and Equiv **)
-
-Definition union (x y : Elem) : WhileL Elem :=
-  bind (ufind x) (fun xVal => bind (ufind y) (fun yVal => link xVal yVal)).
-
-Definition equiv (x y : Elem) : WhileL bool :=
-  bind (ufind x) (fun xVal => bind (ufind y)
-                                  (fun yVal => Return (addr_eqb xVal yVal))).
-  
-(** End of example **)
-
-Definition refineIf' {a} (cond : bool) (pt : PT a) :
-  let branchPre (P : S -> Prop) := fun s => prod (pre pt s) (P s) in
-  let thenBranch := [branchPre (fun s => Is_true cond),
-                     fun s pre s' => post pt s (fst pre) s' ] in
-  let elseBranch := [branchPre (fun s => Is_false cond),
-                     fun s pre s' => post pt s (fst pre) s' ] in
-  (Spec a pt) ⊑ if cond then (Spec a thenBranch) else (Spec a elseBranch).
-Proof.
-  unfold_refinements; destruct cond; simpl;
-  set (d := (fun s pres => pair pres I) : pre pt ⊂ pre ([fun s : S => (pre pt s * True)%type,
-                                        fun (s : S) (pre : pre pt s * True) (s' : a) => post pt s (fst pre) s']));
-  apply (Refinement d); intros; destruct_pt a; auto.
-Defined.
-
-Lemma refineWhilePT' {a} (inv : S -> Prop) (cond : S -> bool) (Q : S -> Prop) : 
-  let pt := [inv , fun s' => inv s' /\ Q s'] in
-  let body : PT a := [fun s => inv s /\ Is_true (cond s), (fun s => inv s)] in
-  (forall s, Is_false (cond s) /\ inv s -> Q s) ->
-  pt ⊏ WhilePT inv cond body.
-  Proof.
-    intros pt body QH; simpl in *.
-    assert (d: pre pt ⊂ pre (WhilePT inv cond body)) by
-      (refine_simpl; repeat split; destruct_conjs; auto).
-    apply (Refinement d).
-    intros; repeat split; refine_simpl; destruct_conjs; now auto.
-Qed.
-
-(* TODO: update this to handle the continuation too
-Lemma refineWhile {a} (inv : S -> Prop) (cond : S -> bool) (Q : S -> Prop) 
-  (StrQ : forall s, Is_false (cond s) /\ inv s -> Q s) : 
-  let w := Spec a ([inv , fun s' => inv s' /\ Q s']) in
-  let body := [fun s => inv s /\ Is_true (cond s), (fun s => inv s)] in
-  w ⊑ While a inv cond (Spec a body).
-  Proof.
-    refine_simpl; now (apply refineWhilePT).
-  Qed.
-*)
-
-
-(* Lemma newSpec {a b : Type} (spec : PT a) (w : Ptr -> WhileL a) (v : b) *)
-(*       (H : forall s, pre spec s -> pre spec (update s (alloc s) (dyn b v))) *)
-(*       (H1 : forall s x v' s0, *)
-(*               post spec (update s (alloc s) (dyn b v)) (H s x) v' s0 -> *)
-(*               post spec s x v' s0) *)
-(*       (Step : forall p,  *)
-(*                 Spec ([ fun s =>  *)
-(*                             {t : S & prod (pre spec s)  *)
-(*                                      (prod (s = update t p (dyn b v)) *)
-(*                                            (p = alloc t)) *)
-(*                                      } *)
-(*                            , fun s pres v s' => post spec s (fst (projT2 pres)) v s' ]) ⊑ w p) : *)
-(*   Spec spec ⊑ New b v w. *)
-(* Proof. *)
-(*   eapply newStep. Unshelve. Focus 2. *)
-(*   * refine_simpl. *)
-(*     exists (alloc s); split; [ apply allocFresh | ]. *)
-(*     destruct (Step (alloc s)) as [d h]. *)
-(*     apply d. *)
-(*     destruct spec. *)
-(*     refine_simpl. *)
-(*     exists s. *)
-(*     split. *)
-(*     now apply H. *)
-(*     split; [ now trivial | reflexivity]. *)
-(*   * refine_simpl; destruct (Step (alloc s)) as [d h]; apply H1. *)
-(*     destruct spec; simpl in *; apply h in X; now simpl in X. *)
-(* Qed. *)
-
-
-
-
-(* SWAP ⊑ (N ::= Var Q ; Q ::= Var P ; P ::= Var N) *)
-(* Definition swapResult (P : Ptr) (Q : Ptr) (D : P <> Q) (a : Type) : *)
-(*   let SetQinN (s : Ptr -> WhileL unit) := *)
-(*       (Read a Q) (fun v => New v s) in *)
-(*   let SetPinQ (s : WhileL unit) := *)
-(*       (Read a P) (fun v => Write Q v s) in *)
-(*   let SetNinP (N : Ptr) (s : WhileL unit) := *)
-(*       (Read a N) (fun v => Write P v s) in *)
-(*   @SWAP a P Q ⊑ SetQinN (fun N => SetPinQ (SetNinP N (Return tt))). *)
-(* Proof. *)
-(*   intros. *)
-(*   unfold SetQinN. *)
-(*   eapply readSpec; refine_simpl. *)
-(*   now exists s1. *)
-(*   eapply newSpec. refine_simpl. *)
-(*   rewrite <- H. *)
-(*   rewrite findAlloc; auto. *)
-(*   apply MFacts.in_find_iff; unfold not; intro HH; *)
-(*   unfold find in H2; rewrite H2 in HH; inversion HH. *)
-(*   rewrite <- H0. *)
-(*   rewrite findNUpdate. *)
-(*   reflexivity. *)
-(*   eapply allocDiff. *)
-(*   apply H1. *)
-  
-(*   intros T; eapply readSpec. *)
-(*   refine_simpl. *)
-(*   now exists s0. *)
-(*   intro vInP. *)
-(*   simpl. *)
-(*   eapply writeSpec. *)
-(*   refine_simpl; eauto. *)
-(*   eapply readSpec. *)
-(*   refine_simpl. *)
-(*   exists v. *)
-(*   rewrite findNUpdate. *)
-(*   rewrite findUpdate. *)
-(*   reflexivity. *)
-(*   rewrite findAlloc in H. *)
-(*   eapply (allocDiff' H). *)
-(*   admit. *)
-(*   refine_simpl. *)
-(*   eapply writeSpec. *)
-(*   refine_simpl; auto. *)
-(*   exists vInP. *)
-(*   rewrite findNUpdate; auto. *)
-(*   apply returnStep; refine_simpl. *)
-(*   unfold preConditionOf in pre; simpl in pre. *)
-(*   destruct_conjs. *)
-(*   simpl; subst. *)
-(*   rewrite e2. *)
-(*   rewrite findNUpdate; auto. *)
-(*   unfold preConditionOf in *. *)
-(*   simpl in *; subst. *)
-(*   destruct_conjs. *)
-(*   simpl. *)
-(*   subst.  *)
-(*   rewrite findUpdate. *)
-(*   rewrite <- e0. *)
-(*   rewrite findNUpdate. *)
-
-  
-(*   rewrite findNUpdate. *)
-(*   assumption. *)
-(*   admit.  *)
-(* (* same admit as above *) *)
-(*   Unshelve. *)
-(*   refine_simpl. *)
-(*   eapply heapGrows. *)
-(*   apply H0. *)
-(*   eapply heapGrows. *)
-(*   apply e. *)
-(*   rewrite findNUpdate. *)
-(*   assumption. *)
-(*   apply (allocDiff (dyn a v)); assumption. *)
-(* Admitted.   *)
-  
-(* (** End of example **) *)
 
 
