Sqrt.v
@@ -36,17 +36,9 @@ Definition Cond (Q R : Ptr) (st : heap nat) :=
   negb (Nat.eqb (find_eqb_some (find st R) + 1)
                 (find_eqb_some (find st Q))).
 
-Lemma ifSpec {a v} (cond : bool) (spec : PT v a) (wt we : WhileL v a) :
-  (if cond then Spec spec ⊑ wt else Spec spec ⊑ we) ->
-  (Spec spec ⊑ (if cond then wt else we)).
-Proof. destruct cond; intros; assumption. Qed.
-
 Hint Unfold isExecutable square.
 Hint Resolve Nat.ltb_lt Lt.lt_n_Sm_le.
 Hint Resolve le_0_n leb_iff_conv beq_nat_eq.
-
-Ltac WHILE I c := apply (whileSpec I c); goal_simpl.
-Ltac ITE c := apply (ifSpec c); remember c as b; destruct b; goal_simpl.
 
 (*** Derivation ***)
 
@@ -68,7 +60,6 @@ Proof.
       repeat (eexists; split; eauto); repeat split; eauto.   
       now apply Nat.ltb_lt.
       WRITE R (Nat.div2 (vInQ + vInR)).
-      eapply (@writeSpec _ _ R (Nat.div2 (vInQ + vInR))); goal_simpl.
       RETURN tt.
       repeat (eexists; split; eauto); repeat split; eauto.
       symmetry in Heqb; apply Lt.lt_n_Sm_le; now apply leb_iff_conv. 
@@ -86,163 +77,6 @@ Defined.
 Variable t : Ptr.
 
 Eval simpl in projT1 (sqrtResult t).
-
-(*** Verification ***)
-
-Definition sqrt (ptr : Ptr) : WhileL nat nat.
-refine (
-  Read ptr (fun s =>
-  New (s + 1) (fun Q =>
-  New 0 (fun R =>
-  While (Inv Q R s)
-        (Cond Q R)
-        (Read Q (fun vInQ =>
-        (Read R (fun vInR =>
-        let p := div2 (vInQ + vInR)
-        in if (s <? square p)
-           then Write Q p (Return _ tt)
-           else Write R p (Return _ tt)))))
-  (Read R (fun vInR => Return _ vInR)))))).
-Defined.
-
-Lemma sqrtRefinement : forall ptr, wrefines (sqrtSpec ptr) (sqrt ptr).
-Proof.
-  intro ptr; unfold sqrtSpec.
-  READ ptr s.
-  NEW (s + 1) Q.
-  NEW 0 R.
-  unfold Inv, Cond; apply whileSpec.
-  - refine_simpl.
-    unfold lift_opt_prop, square; simpl; rewrite findUpdate; simpl; apply le_0_n.
-    unfold square; simpl; rewrite findNUpdate.
-    unfold Nat.lt; rewrite findUpdate; simpl.
-    remember ((s + 1) * (s + 1)).
-    rewrite Nat.add_comm in Heqn1 at 1; simpl in Heqn1.
-    rewrite Nat.add_comm with (m := 1) in Heqn1; rewrite Heqn1.
-    apply Nat.le_add_r.
-    unfold not; intro H'; subst.
-    assert (Ha : R <> R) by eauto; now apply Ha.
-    unfold not; intro H'; subst.
-    assert (Ha : Q <> Q) by eauto; now apply Ha.
-  - READ Q vInQ.
-    remember (find s0 Q).
-    destruct o; [ eauto | exfalso; assumption ].
-    READ R vInR.
-    unfold lift_opt_prop in l.
-    remember (find s0 R) as r; destruct r; [ eauto | exfalso; assumption ].
-    remember (s <? square (Nat.div2 (vInQ + vInR))) as b.
-    destruct b.
-    WRITE Q (Nat.div2 (vInQ + vInR)).
-    RETURN tt;
-    try rewrite findUpdate; try rewrite findNUpdate; auto.
-    rewrite e1 in y; rewrite e0 in l; symmetry in Heqb; now apply Nat.ltb_lt.
-    WRITE R (Nat.div2 (vInQ + vInR)).
-    RETURN tt;
-    try rewrite findUpdate; try rewrite findNUpdate; auto.
-    simpl; symmetry in Heqb; apply leb_iff_conv in Heqb;
-    now apply Lt.lt_n_Sm_le in Heqb.
-  - READ R vInR.
-    unfold lift_opt_prop in l.
-    remember (find s0 R) as r; destruct r; [ eauto | exfalso; assumption ].
-    RETURN vInR.
-    * rewrite e in l; simpl in l; auto.
-    * rewrite e in i; simpl in i.
-      remember (find s0 Q) as q; destruct q.
-      remember (vInR + 1 =? n2) as b; destruct b.
-      apply beq_nat_eq in Heqb.
-      now subst.
-      exfalso; simpl in i; rewrite <- Heqb in i; auto.
-      exfalso; assumption.
-Qed.
-
-(* Refinement with Type *)
-
-Definition lift_opt {a b} (f : a -> a -> b) (v1 : option a) (v2 : option a) : option b :=
-  match v1,v2 with
-    | Some x, Some y => Some (f x y)
-    | _, _ => None
-  end.
-
-Definition sqrt_type (ptr : Ptr) : WhileL nat nat.
-refine (
-  Read ptr (fun s =>
-  New (s + 1) (fun Q =>
-  New 0 (fun R =>
-  While (fun _ st =>
-    prod (lift_opt (fun r s => Nat.leb (square r) s) (find st R) (Some s) = Some true)
-    (prod (lift_opt (fun s q => Nat.ltb s (square q)) (Some s) (find st Q) = Some true) (R <> Q)))
-        (fun st => negb (Nat.eqb (find_eqb_some (find st R) + 1)
-                                 (find_eqb_some (find st Q)))) 
-        (Read Q (fun vInQ =>
-        (Read R (fun vInR =>
-        let p := div2 (vInQ + vInR)
-        in if (s <? square p)
-           then Write Q p (Return _ tt)
-           else Write R p (Return _ tt)))))
-  (Read R (fun vInR => Return _ vInR)))))).
-Defined.
-
-Lemma sqrtRefinement_type : forall ptr, wrefines (sqrtSpec ptr) (sqrt_type ptr).
-Proof.
-  intro ptr; unfold sqrtSpec.
-  READ ptr s.
-  NEW (s + 1) Q.
-  NEW 0 R.
-  apply whileSpec.
-  - refine_simpl.
-    unfold lift_opt, square; simpl; rewrite findUpdate; now simpl.
-    unfold lift_opt, square; simpl. rewrite findNUpdate.
-    unfold Nat.ltb; rewrite findUpdate; simpl.
-    remember ((s + 1) * (s + 1)).
-    rewrite Nat.add_comm in Heqn1. simpl in *.
-    rewrite Heqn1.
-    apply f_equal; apply Nat.leb_le.
-    apply Nat.le_add_r.
-    unfold not; intro H'; subst.
-    assert (Ha : R <> R) by eauto; now apply Ha.
-    unfold not; intro H'; subst.
-    assert (Ha : Q <> Q) by eauto; now apply Ha.
-  - READ Q vInQ.
-    remember (find s0 Q). destruct o. eauto. inversion e0.
-    READ R vInR.
-    unfold lift_opt in e0.
-    remember (find s0 R). destruct o. eauto. inversion e0.
-    remember (s <? square (Nat.div2 (vInQ + vInR))).
-    destruct b.
-    WRITE Q (Nat.div2 (vInQ + vInR)).
-    RETURN tt.
-    rewrite findNUpdate; auto.
-    rewrite findUpdate; apply f_equal.
-    rewrite e0 in e2; rewrite e1 in e3.
-    now rewrite <- Heqb.
-    auto.
-    WRITE R (Nat.div2 (vInQ + vInR)).
-    RETURN tt.
-    rewrite findUpdate; auto.
-    simpl; apply f_equal.
-    symmetry in Heqb.
-    apply leb_iff_conv in Heqb.
-    apply Lt.lt_n_Sm_le in Heqb.
-    now apply Nat.leb_le.
-    rewrite findNUpdate; auto.
-    auto.
-  - READ R vInR.
-    unfold lift_opt in e.
-    remember (find s0 R) as r; destruct r. eauto. inversion e.
-    RETURN vInR.
-    * rewrite e in e0; simpl in e0.
-      inversion e0.  now apply leb_complete in H1.
-    * rewrite e in i.
-      remember (find s0 Q) as q.
-      destruct q; inversion e1. unfold "<?" in H1. unfold lt.
-      apply leb_complete in H1.
-      simpl in i.
-      remember (vInR + 1 =? n2).
-      destruct b.
-      apply beq_nat_eq in Heqb.
-      now subst.
-      exfalso; now simpl in i.
-Qed.
 
     
   
